# Solution to Review Question

by Qiang Gao, updated at Nov 8, 2017

---

## Chapter 2 Large-Sample Theory

### Section 2 Fundamental Concepts in Time-Series Analysis

...

#### Review Question 2.2.3 (No anticipated changes in martingales)

Suppose $$\{ x_i \}$$ is a martingale with respect to $$\{ \mathbf{z}_i \}$$. Show that $$ \operatorname*{E} (x_{i+j} | \mathbf{z}_{i-1}, \mathbf{z}_{i-2}, \ldots, \mathbf{z}_1) = x_{i-1} $$ and $$ \operatorname*{E} (x_{i+j+1} - x_{i+j} | \mathbf{z}_{i-1}, \mathbf{z}_{i-2}, \ldots, \mathbf{z}_1) = 0 $$ for $$ j = 0, 1, \ldots $$

**Hint**: Use the Law of Iterated Expectations.

##### Solution

For $$j = 0, 1, \ldots ,$$

$$
\begin{align*}
\operatorname*{E} (x_{i+j} | \mathbf{z}_{i-1}, \mathbf{z}_{i-2}, \ldots, \mathbf{z}_1)
&= \operatorname*{E} [ \operatorname*{E} (x_{i+j} | \mathbf{z}_{i+j-1}, \mathbf{z}_{i+j-2}, \ldots, \mathbf{z}_1) | \mathbf{z}_{i-1}, \mathbf{z}_{i-2}, \ldots, \mathbf{z}_1]
\\

&= \operatorname*{E} [ x_{i+j-1} | \mathbf{z}_{i-1}, \mathbf{z}_{i-2}, \ldots, \mathbf{z}_1]
\\

&= \operatorname*{E} [ \operatorname*{E} (x_{i+j-1} | \mathbf{z}_{i+j-2}, \mathbf{z}_{i+j-3}, \ldots, \mathbf{z}_1) | \mathbf{z}_{i-1}, \mathbf{z}_{i-2}, \ldots, \mathbf{z}_1]
\\

&= \operatorname*{E} [ x_{i+j-2} | \mathbf{z}_{i-1}, \mathbf{z}_{i-2}, \ldots, \mathbf{z}_1]
\\

&= \cdots
\\

&= \operatorname*{E} [ x_{i} | \mathbf{z}_{i-1}, \mathbf{z}_{i-2}, \ldots, \mathbf{z}_1]
\\

&= x_{i-1}.
\end{align*}
$$

Similarly, $$ \operatorname*{E} (x_{i+j+1} | \mathbf{z}_{i-1}, \mathbf{z}_{i-2}, \ldots, \mathbf{z}_1) = x_{i-1} $$. Combining results,

$$
\begin{align*}
\operatorname*{E} (x_{i+j+1} - x_{i+j} | \mathbf{z}_{i-1}, \mathbf{z}_{i-2}, \ldots, \mathbf{z}_1)
&= \operatorname*{E} (x_{i+j+1} | \mathbf{z}_{i-1}, \mathbf{z}_{i-2}, \ldots, \mathbf{z}_1) - \operatorname*{E} (x_{i+j} | \mathbf{z}_{i-1}, \mathbf{z}_{i-2}, \ldots, \mathbf{z}_1)
\\

&= x_{i-1} - x_{i-1}
\\

&= 0.
\end{align*}
$$

---

Copyright Â©2017 by Qiang Gao